pulse/lib/pulse/core/PulseCore.IndirectionTheorySep.fsti
@@ -187,6 +187,7 @@ val intro_equiv (p: slprop) m : squash (interp (equiv p p) m)
 val equiv_comm (p q: slprop) : squash (equiv p q == equiv q p)
 val equiv_elim p q : squash (equiv p q `star` p == equiv p q `star` q)
 val equiv_trans (p q r: slprop) : squash (equiv p q `star` equiv q r == equiv p q `star` equiv p r)
+val later_equiv (p q: slprop) : squash (later (equiv p q) == equiv (later p) (later q))
 val equiv_timeless (a b: slprop) : Lemma (requires timeless a /\ timeless b) (ensures equiv a b == pure (a == b))
 val equiv_star_congr (p q r: slprop) : squash (equiv q r == equiv q r `star` equiv (star p q) (star p r))
 
